@base <> .
@prefix rdfs: <http://www.w3.org/2000/01/rdf-schema#> .
@prefix rdf: <http://www.w3.org/1999/02/22-rdf-syntax-ns#> .
@prefix xsd: <http://www.w3.org/2001/XMLSchema#> .
@prefix owl: <http://www.w3.org/2002/07/owl#> .

<#ShapeIndex> a owl:Class ;
    rdfs:label "Shape index"@en ;    
    rdfs:comment """The section of the web that the shape index caracterizes.
     It can be a single IRI or IRI pattern in the form of a regex or a set of IRI and/or regex IRI pattern.
      To represent a set multiple `si:subweb` predicate MUST be defined, thus the subweb does not have to be in a tree structure."""@en ;
    owl:equivalentClass [
        a owl:Class ;
        owl:intersectionOf (
            [ a owl:Restriction ;
              owl:onProperty <#subweb> ;
              owl:minQualifiedCardinality "1"^^xsd:nonNegativeInteger 
            ]
            [ a owl:Restriction ;
              owl:onProperty <#complete> ;
              owl:minQualifiedCardinality "0"^^xsd:nonNegativeInteger ;
              owl:maxQualifiedCardinality "1"^^xsd:nonNegativeInteger 
            ]
            [ a owl:Restriction ;
              owl:onProperty <#entry> ;
              owl:minQualifiedCardinality "1"^^xsd:nonNegativeInteger 
            ]
        )                             
    ] .

<#Entry> a owl:Class ;
    rdfs:label "Entry"@en ;
    rdfs:comment "A shape index entry mapping a shape of resources to an RDF shape."@en ; 
    owl:equivalentClass [
        a owl:Class ;
        owl:intersectionOf (
            [ a owl:Restriction ;
              owl:onProperty <#subweb> ;
              owl:minQualifiedCardinality "1"^^xsd:nonNegativeInteger
            ]
            [ a owl:Restriction ;
              owl:onProperty <#excludes> ;
              owl:minQualifiedCardinality "0"^^xsd:nonNegativeInteger ;
              owl:maxQualifiedCardinality "1"^^xsd:nonNegativeInteger
            ]
            [ a owl:Restriction ;
              owl:onProperty <#shape> ;
              owl:qualifiedCardinality "1"^^xsd:nonNegativeInteger
            ]
        )                             
    ] .

<#entry> a owl:ObjectProperty ;
    rdfs:label "Has an entry"@en ;
    rdfs:comment "Lead to a `si:Entry` in the object position."@en ;
    rdfs:domain <#ShapeIndex>;
    rdfs:range <#Entry> .

<#shapeIndexLocation> a owl:ObjectProperty ;
    rdfs:label "A shape index is located at"@en ;
    rdfs:comment "Indicate that a shape index is located at the IRI at the object position of a triple using this term at the predicate position."@en ;
    rdfs:range <#ShapeIndex> .

<#subweb> a  owl:ObjectProperty ;
    rdfs:label "Is within this subweb"@en ;
    rdfs:comment """The section of the web that the shape index caracterizes.
      It can be a single IRI or IRI pattern in the form of a regex or a set of IRI and/or regex IRI pattern.
      To represent a set multiple `si:subweb` predicate MUST be defined, thus the subweb does not have to be
      in a tree structure."""@en ;
    rdfs:domain <#ShapeIndex>;
    rdfs:domain <#Entry>;
    rdfs:range [
        a owl:Class ;
        owl:unionOf ( xsd:string rdfs:Resource )
    ] .

<#complete> a  owl:ObjectProperty ;
    rdfs:label "Is the shape index complete"@en ;
    rdfs:comment "A flag indicating if a shape index is complete, thus, every resource inside the subweb is describe by the index."@en;
    rdfs:domain <#ShapeIndex>;
    rdfs:range xsd:boolean .

<#shape> a  owl:ObjectProperty ;
    rdfs:label "Is validated by the shape"@en ;
    rdfs:comment "The shape binding a `si:subweb`."@en;
    rdfs:domain <#Entry> ;
    rdfs:range rdfs:Resource .

<#excludes> a  owl:ObjectProperty ;
    rdfs:label "Is the shape excluded from the subweb"@en ;
    rdfs:comment "Indicate that the `si:Entry` exclude the shape from the target subweb."@en;
    rdfs:domain <#ShapeIndex>;
    rdfs:range xsd:boolean .

<#indexSubweb> a <#subweb> ;
    rdfs:label "Subweb of the shape index"@en ;
    rdfs:comment "Indicate that the subweb of the entry is the whole subweb of the shape index"@en.

<http://www.w3.org/ns/solid/terms#instanceContainer> a <#subweb> ;
  rdfs:comment """When a Solid container is used as a subweb, the resources are distributed following the LDP Specification.
  See the Solid Specification for more information https://solidproject.org/TR/protocol and 
  the Type Index Specification https://solid.github.io/type-indexes/"""@en.